MonadBind/Monad.v
@@ -78,54 +78,48 @@ repeat (monad'; repeat match goal with
     | |- context [match ?x with _ => _ end] => destruct x
 end; monad'); try (unfold compose, id; cbn; congruence; fail).
 
-Section Lifts.
+(*Section Lifts.
 
 Variable M : Type -> Type.
 Variable inst : Monad M.
 Variables A B C D E F : Type.
 
-Definition liftM
-    (f : A -> B)
-    (ma : M A) : M B :=
-    ma >>= fun a : A => ret (f a).
-
 Definition liftM2
-    (f : A -> B -> C)
-    (ma : M A) (mb : M B) : M C :=
-    ma >>= fun a : A =>
-    mb >>= fun b : B => ret (f a b).
+  (f : A -> B -> C)
+  (ma : M A) (mb : M B) : M C :=
+  ma >>= fun a : A =>
+  mb >>= fun b : B => ret (f a b).
 
 Definition liftM3
-    (f : A -> B -> C -> D)
-    (ma : M A) (mb : M B) (mc : M C) : M D :=
-    ma >>= fun a : A =>
-    mb >>= fun b : B => 
-    mc >>= fun c : C => ret (f a b c).
+  (f : A -> B -> C -> D)
+  (ma : M A) (mb : M B) (mc : M C) : M D :=
+  ma >>= fun a : A =>
+  mb >>= fun b : B => 
+  mc >>= fun c : C => ret (f a b c).
 
 Definition liftM4
-    (f : A -> B -> C -> D -> E)
-    (ma : M A) (mb : M B) (mc : M C) (md : M D) : M E :=
-    ma >>= fun a : A =>
-    mb >>= fun b : B =>
-    mc >>= fun c : C =>
-    md >>= fun d : D => ret (f a b c d).
+  (f : A -> B -> C -> D -> E)
+  (ma : M A) (mb : M B) (mc : M C) (md : M D) : M E :=
+  ma >>= fun a : A =>
+  mb >>= fun b : B =>
+  mc >>= fun c : C =>
+  md >>= fun d : D => ret (f a b c d).
 
 Definition liftM5
-    (f : A -> B -> C -> D -> E -> F)
-    (ma : M A) (mb : M B) (mc : M C) (md : M D) (me : M E) : M F :=
-    ma >>= fun a : A =>
-    mb >>= fun b : B =>
-    mc >>= fun c : C =>
-    md >>= fun d : D =>
-    me >>= fun e : E => ret (f a b c d e).
+  (f : A -> B -> C -> D -> E -> F)
+  (ma : M A) (mb : M B) (mc : M C) (md : M D) (me : M E) : M F :=
+  ma >>= fun a : A =>
+  mb >>= fun b : B =>
+  mc >>= fun c : C =>
+  md >>= fun d : D =>
+  me >>= fun e : E => ret (f a b c d e).
 
 End Lifts.
-Check liftM2.
-Arguments liftM [M inst A B] _ _.
+
 Arguments liftM2 [M inst A B C] _ _ _.
 Arguments liftM3 [M inst A B C D] _ _ _ _.
 Arguments liftM4 [M inst A B C D E] _ _ _ _ _.
-Arguments liftM5 [M inst A B C D E F] _ _ _ _ _ _.
+Arguments liftM5 [M inst A B C D E F] _ _ _ _ _ _.*)
 
 Section MonadicFuns.
 
@@ -133,12 +127,7 @@ Variable M : Type -> Type.
 Variable inst : Monad M.
 Variables A B C D E F : Type.
 
-(* TODO remove after Applicative is superclass of Monad. *)
-(*Definition ap (mf : M (A -> B)) (ma : M A) : M B :=
-    mf >>= fun f =>
-    ma >>= fun a => ret (f a).*)
-
-Fixpoint filterM (f : A -> M bool) (la : list A) : M (list A) :=
+(*Fixpoint filterM (f : A -> M bool) (la : list A) : M (list A) :=
 match la with
     | [] => ret []
     | h :: t => f h >>= fun b : bool => if b
@@ -165,7 +154,7 @@ match la, lb with
     | [], _ => ret []
     | _, [] => ret []
     | ha :: ta, hb :: tb => liftM2 (@cons C) (f ha hb) (zipWithM f ta tb)
-end.
+end.*)
 
 Fixpoint foldM (f : A -> B -> M A) (dflt : A) (l : list B)
     : M A :=
@@ -174,42 +163,41 @@ match l with
     | h :: t => f dflt h >>= fun a : A => foldM f a t
 end.
 
-Definition when (b : bool) (mu : M unit) : M unit :=
+(*Definition when (b : bool) (mu : M unit) : M unit :=
 match b with
     | true => mu
     | false => ret tt
 end.
 
 Definition unless (b : bool) (mu : M unit) : M unit :=
-    when (negb b) mu.
+    when (negb b) mu.*)
 
 End MonadicFuns.
 
-(*Arguments ap [M] [inst] [A] [B] _ _.*)
-Arguments filterM [M] [inst] [A] _ _.
+(*Arguments filterM [M] [inst] [A] _ _.
 Arguments sequence [M] [inst] [A] _.
 Arguments replicateM [M] [inst] [A] _ _.
-Arguments zipWithM [M] [inst] [A] [B] [C] _ _ _.
+Arguments zipWithM [M] [inst] [A] [B] [C] _ _ _.*)
 Arguments foldM [M] [inst] [A] [B] _ _ _.
-Arguments when [M] [inst] _ _.
-Arguments unless [M] [inst] _ _.
+(*Arguments when [M] [inst] _ _.
+Arguments unless [M] [inst] _ _.*)
 
-Section MonadicFuns2.
+(*Section MonadicFuns2.
 
 Variable M : Type -> Type.
 Variable inst : Monad M.
 Variables A B C D E F : Type.
 
 Definition mapM (f : A -> M B) (la : list A) : M (list B) :=
-    sequence (fmap f la).
+  sequence (fmap f la).
 
 Definition forM (la : list A) (f : A -> M B) : M (list B) :=
-    mapM f la.
+  mapM f la.
 
 End MonadicFuns2.
 
 Arguments mapM [M] [inst] [A] [B] _ _.
-Arguments forM [M] [inst] [A] [B] _ _.
+Arguments forM [M] [inst] [A] [B] _ _.*)
 
 Section DerivedLaws.
 
@@ -267,13 +255,3 @@ Proof.
 Qed.
 
 End DerivedLaws.
-
-(* TODO: add this to other definitions of monads *)
-Module wut.
-
-Notation "f $$ x" := (ap f x)
-  (left associativity, at level 40, only parsing).
-
-End wut.
-
-Export wut.
